Implemented the protocol. Not proven yet.

impl.c
@@ -1,0 +1,40 @@
+﻿#include "dist/impl/Impl_NeedSchr.h"
+
+#include <Hacl_NaCl.h>
+#include <Lib_RandomBuffer_System.h>
+
+#include <stdlib.h>
+
+void Impl_NeedSchr_new_key(uint8_t *r){
+    Lib_RandomBuffer_System_crypto_random(r, KEY_LENGTH);
+}
+
+void Impl_NeedSchr_new_host(uint8_t *r){
+    Lib_RandomBuffer_System_crypto_random(r, HOST_LENGTH);
+}
+
+void Impl_NeedSchr_new_nonce(uint8_t *r){
+    Lib_RandomBuffer_System_crypto_random(r, NONCE_LENGTH);
+}
+
+void Impl_NeedSchr_encrypt(uint8_t *k, uint8_t *p, uint8_t *c, uint32_t l){
+    // We prefix ciphertext with nonce.
+    Impl_NeedSchr_new_nonce(c);
+
+    if(Hacl_NaCl_crypto_secretbox_easy(c+NONCE_LENGTH, p, l-CIPHER_HEADER_LENGTH, c, k) != 0){
+        // This should never happen.
+        abort();
+    }
+}
+
+bool Impl_NeedSchr_decrypt(uint8_t *k, uint8_t *c, uint8_t *p, uint32_t l){
+    return Hacl_NaCl_crypto_secretbox_open_easy(p, c+NONCE_LENGTH, l-NONCE_LENGTH, c, k) == 0;
+}
+
+void Impl_NeedSchr_dec(uint8_t *n){
+    for(size_t i = 0;i < NONCE_LENGTH;++i){
+        if(n[i]-- != 0){
+            break;
+        }
+    }
+}
