main.c
@@ -1,7 +1,64 @@
-﻿#include <stdio.h>
+﻿// We always want assertions.
+#undef NDEBUG
+
+#include <stdio.h>
+#include <assert.h>
 
 #include "dist/impl/Impl_NeedSchr.h"
 
 int main(){
-    // printf("%u\n",Impl_NeedSchr_mul(6,7));
+    uint8_t a[HOST_LENGTH];
+    Impl_NeedSchr_new_host(a);
+
+    uint8_t b[HOST_LENGTH];
+    Impl_NeedSchr_new_host(b);
+
+    uint8_t kAS[KEY_LENGTH];
+    Impl_NeedSchr_new_key(kAS);
+
+    uint8_t kBS[KEY_LENGTH];
+    Impl_NeedSchr_new_key(kBS);
+
+    uint8_t nA[NONCE_LENGTH];
+    Impl_NeedSchr_new_nonce(nA);
+
+    uint8_t state1_A[STATE1_A_LENGTH];
+    uint8_t m1[M1_LENGTH];
+    Impl_NeedSchr_initiate_A(kAS, a, b, nA, state1_A, m1);
+    // A -> S: (a, b, nA)
+    uint8_t kAB[KEY_LENGTH];
+    Impl_NeedSchr_new_key(kAB);
+
+    uint8_t m2[M2_LENGTH];
+    uint8_t a_S[HOST_LENGTH];
+    Impl_NeedSchr_generate_key_S(kAS, kBS, m1, kAB, m2, a_S);
+
+    assert(memcmp(a, a_S, HOST_LENGTH) == 0);
+
+    // S -> A: { nA, kAB, b, { kAB, a }kBS }kAS
+    uint8_t state2_A[STATE2_A_LENGTH];
+    uint8_t m3[M3_LENGTH];
+    assert(Impl_NeedSchr_handshake_A(state1_A, m2, state2_A, m3));
+
+    // A -> B: { kAB, a }kBS
+    uint8_t nB[NONCE_LENGTH];
+    Impl_NeedSchr_new_nonce(nB);
+
+    uint8_t state_B[STATE_B_LENGTH];
+    uint8_t m4[M4_LENGTH];
+    uint8_t a_B[HOST_LENGTH];
+    assert(Impl_NeedSchr_handshake_B(kBS, m3, nB, state_B, m4, a_B));
+
+    assert(memcmp(a, a_B, HOST_LENGTH) == 0);
+
+    // B -> A: { nB }kAB
+    uint8_t m5[M5_LENGTH];
+    uint8_t kAB_A[KEY_LENGTH];
+    assert(Impl_NeedSchr_accept_A(state2_A, m4, kAB_A, m5));
+
+    // A -> B: { dec(nB) }kAB
+    uint8_t kAB_B[KEY_LENGTH];
+    assert(Impl_NeedSchr_accept_B(state_B, m5, kAB_B));
+
+    assert(memcmp(kAB_A, kAB_B, KEY_LENGTH) == 0);
 }
