fstar/Impl.NeedSchr.fst
@@ -6,11 +6,13 @@ module U32 = FStar.UInt32
 module S = FStar.Seq
 module B = LowStar.Buffer
 module M = LowStar.Modifies
+module H = FStar.HyperStack
 module ST = FStar.HyperStack.ST
 
 module Spec = Spec.NeedSchr
 
 open FStar.HyperStack.ST
+open LowStar.BufferOps
 open Memcpy
 
 // open Lib.RandomBuffer.System
@@ -28,11 +30,15 @@ noextract inline_for_extraction let state1_A_length = U32.(key_length +^ host_le
 noextract inline_for_extraction let state2_A_length = key_length
 noextract inline_for_extraction let state_B_length = U32.(key_length +^ nonce_length)
 
-noextract inline_for_extraction let message1_length = U32.(host_length +^ host_length +^ nonce_length)
-noextract inline_for_extraction let message3_length = U32.(cipher_header_length +^ key_length +^ host_length)
-noextract inline_for_extraction let message2_length = U32.(cipher_header_length +^ nonce_length +^ key_length +^ host_length +^ message3_length)
-noextract inline_for_extraction let message4_length = U32.(cipher_header_length +^ nonce_length)
-noextract inline_for_extraction let message5_length = U32.(cipher_header_length +^ nonce_length)
+noextract inline_for_extraction let m1_length = U32.(host_length +^ host_length +^ nonce_length)
+noextract inline_for_extraction let m3_length = U32.(cipher_header_length +^ key_length +^ host_length)
+noextract inline_for_extraction let m2_length = U32.(cipher_header_length +^ nonce_length +^ key_length +^ host_length +^ m3_length)
+noextract inline_for_extraction let m4_length = U32.(cipher_header_length +^ nonce_length)
+noextract inline_for_extraction let m5_length = U32.(cipher_header_length +^ nonce_length)
+
+noextract inline_for_extraction let state1_A_kAS = 0ul
+noextract inline_for_extraction let state1_A_b   = U32.(state1_A_kAS +^ key_length)
+noextract inline_for_extraction let state1_A_nA  = U32.(state1_A_b   +^ host_length)
 
 noextract inline_for_extraction type key   = b: B.buffer U8.t{B.length b = U32.v key_length}
 noextract inline_for_extraction type host  = b: B.buffer U8.t{B.length b = U32.v host_length}
@@ -42,36 +48,36 @@ noextract inline_for_extraction type state1_At = b: B.buffer U8.t{B.length b = U
 noextract inline_for_extraction type state2_At = b: B.buffer U8.t{B.length b = U32.v state2_A_length}
 noextract inline_for_extraction type state_Bt  = b: B.buffer U8.t{B.length b = U32.v state_B_length}
 
-noextract inline_for_extraction type m1t = b: B.buffer U8.t{B.length b = U32.v message1_length}
-noextract inline_for_extraction type m3t = b: B.buffer U8.t{B.length b = U32.v message3_length}
-noextract inline_for_extraction type m2t = b: B.buffer U8.t{B.length b = U32.v message2_length}
-noextract inline_for_extraction type m4t = b: B.buffer U8.t{B.length b = U32.v message4_length}
-noextract inline_for_extraction type m5t = b: B.buffer U8.t{B.length b = U32.v message5_length}
+noextract inline_for_extraction type m1t = b: B.buffer U8.t{B.length b = U32.v m1_length}
+noextract inline_for_extraction type m2t = b: B.buffer U8.t{B.length b = U32.v m2_length}
+noextract inline_for_extraction type m3t = b: B.buffer U8.t{B.length b = U32.v m3_length}
+noextract inline_for_extraction type m4t = b: B.buffer U8.t{B.length b = U32.v m4_length}
+noextract inline_for_extraction type m5t = b: B.buffer U8.t{B.length b = U32.v m5_length}
+
+noextract inline_for_extraction let m1_a = 0ul
+noextract inline_for_extraction let m1_b = U32.(m1_a +^ host_length)
+noextract inline_for_extraction let m1_nA = U32.(m1_b +^ host_length)
+
+noextract inline_for_extraction let m2_nA = 0ul
+noextract inline_for_extraction let m2_kAB = U32.(m2_nA +^ nonce_length)
+noextract inline_for_extraction let m2_b = U32.(m2_kAB +^ key_length)
+noextract inline_for_extraction let m2_m3 = U32.(m2_b +^ host_length)
+
+noextract inline_for_extraction let m3_kAB = 0ul
+noextract inline_for_extraction let m3_a = U32.(m3_kAB +^ key_length)
+
+noextract inline_for_extraction let state_B_kAB = 0ul
+noextract inline_for_extraction let state_B_nB = U32.(state_B_kAB +^ key_length)
 
 assume val new_key: (r: key) -> EXT unit
 assume val new_host: (r: host) -> EXT unit
 assume val new_nonce: (r: nonce) -> EXT unit
-
-effect Mem (a: Type) (b: B.buffer U8.t) = Stack a
-    (requires fun h -> B.live h b)
-    (ensures  fun h0 _ h1 -> ST.modifies_none h0 h1)
 
 noextract let join3 (l1, l2, l3: (S.seq 'a & S.seq 'a & S.seq 'a))
     = S.(l1 @| l2 @| l3)
 
 noextract let join4 (l1, l2, l3, l4: (S.seq 'a & S.seq 'a & S.seq 'a & S.seq 'a))
     = S.(l1 @| l2 @| l3 @| l4)
-
-(*
-type m3t = ciphertext (key & host)
-type m2t =  ciphertext (nonce & key & host & m3t)
-*)
-noextract let joinCipher (v:Spec.m2t) =
-    let _, t = v in
-    let n, k, h, m3 = t in
-    let _, tt = m3 in
-    let inner_key, inner_host = tt in 
-    S.(n @| k @| h @|  inner_key @| inner_host)
 
 #push-options "--z3rlimit 10"
 let initiate_A (kAS: key) (a b: host) (nA: nonce) (state: state1_At) (m1: m1t): Stack unit
@@ -92,15 +98,308 @@ let initiate_A (kAS: key) (a b: host) (nA: nonce) (state: state1_At) (m1: m1t): 
 =
     let open U32 in
     // state
-    memcpy kAS (B.sub state 0ul key_length) key_length;
-    memcpy b   (B.sub state key_length host_length) host_length;
-    memcpy nA  (B.sub state (key_length +^ host_length) nonce_length) nonce_length;
+    memcpy kAS (B.sub state state1_A_kAS key_length)   key_length;
+    memcpy b   (B.sub state state1_A_b   host_length)  host_length;
+    memcpy nA  (B.sub state state1_A_nA  nonce_length) nonce_length;
     // m1
-    memcpy a  (B.sub m1 0ul host_length) host_length;
-    memcpy b  (B.sub m1 host_length host_length) host_length;
-    memcpy nA (B.sub m1 (host_length +^ host_length) nonce_length) nonce_length;
+    memcpy a  (B.sub m1 m1_a  host_length)  host_length;
+    memcpy b  (B.sub m1 m1_b  host_length)  host_length;
+    memcpy nA (B.sub m1 m1_nA nonce_length) nonce_length;
     ()
 #pop-options
+
+let encrypt_pre (k: key) (p c: B.buffer U8.t) (l: U32.t{l `U32.gt` cipher_header_length}) (h: H.mem) =
+    let open B in
+    B.length p = U32.v U32.(l -^ cipher_header_length) /\
+    B.length c = U32.v l /\
+    live h k /\ live h p /\ live h c /\
+    True
+
+assume val encrypt:
+    k: key ->
+    p: B.buffer U8.t ->
+    c: B.buffer U8.t ->
+    l: U32.t{l `U32.gt` cipher_header_length} ->
+    Stack unit
+    (requires fun h ->
+        let open B in
+        encrypt_pre k p c l h /\
+        disjoint c k /\ disjoint c p /\
+        True)
+    (ensures fun h0 _ h1 ->
+        let open B in
+        modifies (loc_buffer c) h0 h1 /\
+        // plaintext_of and key_of
+        True)
+
+assume val decrypt:
+    k: key ->
+    c: B.buffer U8.t ->
+    p: B.buffer U8.t ->
+    l: U32.t{l `U32.gt` cipher_header_length} ->
+    Stack bool
+    (requires fun h ->
+        let open B in
+        encrypt_pre k p c l h /\
+        disjoint p k /\ disjoint p c /\
+        True)
+    // (requires fun _ -> True)
+    (ensures fun h0 b h1 ->
+        let open B in
+        modifies (loc_buffer p) h0 h1 /\
+        // plaintext_of and key_of
+        True)
+
+noextract inline_for_extraction let nul = U8.uint_to_t 0
+
+// This may not be feasible prove.
+#push-options "--z3rlimit 60"
+let generate_key_S (kAS kBS: key) (m1: m1t) (kAB: key) (m2: m2t) (a: host): Stack unit
+    (requires fun h ->
+        let open B in
+        live h kAS /\ live h kBS /\ live h m1 /\ live h kAB /\ live h m2 /\ live h a /\
+        disjoint m2 kAS /\ disjoint m2 kBS /\ disjoint m2 m1 /\ disjoint m2 kAB /\
+        disjoint a kAS /\ disjoint a kBS /\ disjoint a m1 /\ disjoint a kAB /\
+        disjoint a m2)
+    (ensures fun h0 _ h1 ->
+        let open M in
+        // modifies (loc_union (loc_buffer m2) (loc_buffer a)) h0 h1 /\
+        // TODO: Prove.
+        True)
+=
+    push_frame();
+    let open U32 in
+    // m1
+    memcpy (B.sub m1 m1_a host_length) a host_length;
+    let b  = B.sub m1 m1_b  host_length in
+    let nA = B.sub m1 m1_nA nonce_length in
+    // m3
+    let m3_p = B.alloca nul (m3_length -^ cipher_header_length) in
+    memcpy kAB (B.sub m3_p m3_kAB key_length) key_length;
+    memcpy a   (B.sub m3_p m3_a host_length)  host_length;
+    // m2
+    let m2_p = B.alloca nul (m2_length -^ cipher_header_length) in
+    memcpy nA  (B.sub m2_p m2_nA nonce_length) nonce_length;
+    memcpy kAB (B.sub m2_p m2_kAB key_length)  key_length;
+    memcpy b   (B.sub m2_p m2_b host_length)   host_length;
+    encrypt kBS m3_p (B.sub m2_p m2_m3 m3_length) m3_length;
+    encrypt kAS m2_p m2 m2_length;
+    pop_frame()
+#pop-options
+
+noextract inline_for_extraction let host_eq (b1: host) (b2: host): Stack bool
+    (requires fun h ->
+        let open B in
+        live h b1 /\ live h b2)
+    (ensures fun h0 r h1 ->
+        let open B in
+        modifies loc_none h0 h1 /\
+        r <==> (B.as_seq h0 b1 `S.equal` B.as_seq h0 b2) /\
+        True)
+=
+    assert (host_length = 6ul);
+    let r0 = b1.(0ul) = b2.(0ul) in
+    let r1 = b1.(1ul) = b2.(1ul) in
+    let r2 = b1.(2ul) = b2.(2ul) in
+    let r3 = b1.(3ul) = b2.(3ul) in
+    let r4 = b1.(4ul) = b2.(4ul) in
+    let r5 = b1.(5ul) = b2.(5ul) in
+    r0 && r1 && r2 && r3 && r4 && r5
+
+noextract inline_for_extraction let nonce_eq (b1: nonce) (b2: nonce): Stack bool
+    (requires fun h ->
+        let open B in
+        live h b1 /\ live h b2)
+    (ensures fun h0 r h1 ->
+        let open B in
+        modifies loc_none h0 h1 /\
+        r <==> (B.as_seq h0 b1 `S.equal` B.as_seq h0 b2) /\
+        True)
+=
+    assert (nonce_length = 24ul);
+    let r0  = b1.( 0ul) = b2.( 0ul) in
+    let r1  = b1.( 1ul) = b2.( 1ul) in
+    let r2  = b1.( 2ul) = b2.( 2ul) in
+    let r3  = b1.( 3ul) = b2.( 3ul) in
+    let r4  = b1.( 4ul) = b2.( 4ul) in
+    let r5  = b1.( 5ul) = b2.( 5ul) in
+    let r6  = b1.( 6ul) = b2.( 6ul) in
+    let r7  = b1.( 7ul) = b2.( 7ul) in
+    let r8  = b1.( 8ul) = b2.( 8ul) in
+    let r9  = b1.( 9ul) = b2.( 9ul) in
+    let r10 = b1.(10ul) = b2.(10ul) in
+    let r11 = b1.(11ul) = b2.(11ul) in
+    let r12 = b1.(12ul) = b2.(12ul) in
+    let r13 = b1.(13ul) = b2.(13ul) in
+    let r14 = b1.(14ul) = b2.(14ul) in
+    let r15 = b1.(15ul) = b2.(15ul) in
+    let r16 = b1.(16ul) = b2.(16ul) in
+    let r17 = b1.(17ul) = b2.(17ul) in
+    let r18 = b1.(18ul) = b2.(18ul) in
+    let r19 = b1.(19ul) = b2.(19ul) in
+    let r20 = b1.(20ul) = b2.(20ul) in
+    let r21 = b1.(21ul) = b2.(21ul) in
+    let r22 = b1.(22ul) = b2.(22ul) in
+    let r23 = b1.(23ul) = b2.(23ul) in
+     r0 &&  r1 &&  r2 &&  r3 &&  r4 &&  r5 &&  r6 &&  r7 &&  r8 &&  r9 &&
+    r10 && r11 && r12 && r13 && r14 && r15 && r16 && r17 && r18 && r19 &&
+    r20 && r21 && r22 && r23
+
+#push-options "--z3rlimit 30"
+let handshake_A (state1: state1_At) (m2: m2t) (state2: state2_At) (m3: m3t): Stack bool
+    (requires fun h ->
+        let open B in
+        live h state1 /\ live h m2 /\ live h state2 /\ live h m3 /\
+        disjoint state2 state1 /\ disjoint state2 m2 /\
+        disjoint m3 state1 /\ disjoint m3 m2 /\
+        disjoint state2 m3)
+    (ensures fun h0 _ h1 ->
+        let open M in
+        // modifies (loc_union (loc_buffer state2) (loc_buffer m3)) h0 h1 /\
+        // TODO: Prove.
+        True)
+=
+    push_frame();
+    let open U32 in
+    // state
+    let kAS = B.sub state1 state1_A_kAS key_length in
+    // m2
+    let m2_p = B.alloca nul (m2_length -^ cipher_header_length) in
+    let r = if decrypt kAS m2 m2_p m2_length then
+        let b  = B.sub state1 state1_A_b  host_length in
+        let nA = B.sub state1 state1_A_nA nonce_length in
+        let b'  = B.sub m2_p m2_b  host_length in
+        let nA' = B.sub m2_p m2_nA nonce_length in
+        let eq_b = host_eq b b' in
+        let eq_nA = nonce_eq nA nA' in
+        if eq_b && eq_nA then (
+            // state2
+            memcpy (B.sub m2_p m2_kAB key_length) state2 key_length;
+            // m3
+            memcpy (B.sub m2_p m2_m3  m3_length)  m3 m3_length;
+            true)
+        else false
+    else false in
+    pop_frame();
+    r
+#pop-options
+
+assume val dec: n: nonce -> Stack unit
+    (requires fun h ->
+        let open B in
+        live h n)
+    (ensures fun h0 _ h1 ->
+        let open M in
+        modifies (loc_buffer n) h0 h1 /\
+        True)
+
+#push-options "--z3rlimit 30"
+let handshake_B (kBS: key) (m3: m3t) (nB: nonce) (state: state_Bt) (m4: m4t) (a: host): Stack bool
+    (requires fun h ->
+        let open B in
+        live h kBS /\ live h m3 /\ live h nB /\ live h state /\ live h m4 /\ live h a /\
+        disjoint state kBS /\ disjoint state m3 /\ disjoint state nB /\
+        disjoint m4 kBS /\ disjoint m4 m3 /\ disjoint m4 nB /\
+        disjoint a kBS /\ disjoint a m3 /\ disjoint a nB /\
+        disjoint state m4 /\ disjoint state a /\ disjoint m4 a)
+    (ensures fun h0 _ h1 ->
+        let open M in
+        // modifies (loc_union (loc_buffer state) (loc_buffer m4) (loc_buffer a)) h0 h1 /\
+        // TODO: Prove.
+        True)
+=
+    push_frame();
+    let open U32 in
+    // m3
+    let m3_p = B.alloca nul (m3_length -^ cipher_header_length) in
+    let r = if decrypt kBS m3 m3_p m3_length then (
+        let kAB = B.sub m3_p m3_kAB key_length in
+        // state
+        memcpy kAB (B.sub state state_B_kAB key_length)   key_length;
+        memcpy nB  (B.sub state state_B_nB  nonce_length) nonce_length;
+        // m4
+        encrypt kAB nB m4 m4_length;
+        // a
+        memcpy (B.sub m3_p m3_a host_length) a host_length;
+        true)
+    else false in
+    pop_frame();
+    r
+#pop-options
+
+#push-options "--z3rlimit 30"
+let accept_A (state: state2_At) (m4: m4t) (kAB: key) (m5: m5t): Stack bool
+    (requires fun h ->
+        let open B in
+        live h state /\ live h m4 /\ live h m5 /\ live h kAB /\
+        disjoint kAB state /\ disjoint kAB m4 /\
+        disjoint m5 state /\ disjoint m5 m4 /\
+        disjoint kAB m5)
+    (ensures fun h0 _ h1 ->
+        let open M in
+        modifies (loc_union (loc_buffer m5) (loc_buffer kAB)) h0 h1 /\
+        // TODO: Prove.
+        True)
+=
+    push_frame();
+    let open U32 in
+    // m4
+    let m4_p = B.alloca nul (m4_length -^ cipher_header_length) in
+    let r = if decrypt state m4 m4_p m4_length then (
+        let nB = m4_p in
+        dec nB;
+        // kAB
+        memcpy state kAB key_length;
+        // m5
+        encrypt kAB nB m5 m5_length;
+        true)
+    else false in
+    pop_frame();
+    r
+#pop-options
+
+#push-options "--z3rlimit 30"
+let accept_B (state: state_Bt) (m5: m5t) (kAB: key): Stack bool
+    (requires fun h ->
+        let open B in
+        live h state /\ live h m5 /\ live h kAB /\
+        disjoint kAB state /\ disjoint kAB m5)
+    (ensures fun h0 _ h1 ->
+        let open M in
+        // modifies (loc_buffer kAB) h0 h1 /\
+        // TODO: Prove.
+        True)
+=
+    push_frame();
+    let open U32 in
+    // m5
+    let kAB' = B.sub state state_B_kAB key_length in
+    let m5_p = B.alloca nul (m5_length -^ cipher_header_length) in
+    let r = if decrypt kAB' m5 m5_p m5_length then (
+        let nB  = B.sub state state_B_nB  nonce_length in
+        let nB' = B.alloca nul nonce_length in
+        memcpy nB nB' nonce_length;
+        dec nB';
+        // kAB
+        if nonce_eq nB' m5_p then (
+            memcpy kAB' kAB key_length;
+            true)
+        else false)
+    else false in
+    pop_frame();
+    r
+#pop-options
+
+(*
+type m3t = ciphertext (key & host)
+type m2t =  ciphertext (nonce & key & host & m3t)
+*)
+noextract let joinCipher (v: Spec.m2t) =
+    let _, t = v in
+    let n, k, h, m3 = t in
+    let _, tt = m3 in
+    let inner_key, inner_host = tt in
+    S.(n @| k @| h @|  inner_key @| inner_host)
 
 noextract let toSeq (l1: (S.seq 'a))
     = S.(l1)
@@ -117,7 +416,7 @@ noextract let toSeq (l1: (S.seq 'a))
 
 #push-options "--z3rlimit 10"
 let handshake_A (kAS, b, nA: state1_At) (m2: m2t) (state: state2_At) (m3: m3t) =
-(requires fun h -> 
+(requires fun h ->
     let open B in
     live h kAS /\ live h b /\ live h nA /\ live h m2 /\
     disjoint state kAS /\ disjoint state b /\ disjoint state nA /\ disjoint state m2 /\
@@ -153,10 +452,10 @@ let generate_key_S (kAS kBS kAB: key) (a b:host) (nA:nonce) (*(m1:m1t)*) (m2: m2
         modifies (loc_union (loc_buffer m2) (loc_buffer e)) h0 h1  (* modifies l (abstract location) h0 (initial heap) h1(resulting heap) *) /\
         B.as_seq h1 e `S.equal` toSeq e' /\
         B.as_seq h1 m2 `S.equal` joinCipher m2' /\
-        
+
         (*
         type m2t = ciphertext (nonce & key & host & m3t)
-            
+
             should encrypt but we cannot use hacl?
         *)
         True
